<?xml version="1.0"?>
<rdf:RDF xmlns="https://www.w3id.org/iSeeOnto/BehaviourTreeExecution#"
     xml:base="https://www.w3id.org/iSeeOnto/BehaviourTreeExecution"
     xmlns:owl="http://www.w3.org/2002/07/owl#"
     xmlns:rdf="http://www.w3.org/1999/02/22-rdf-syntax-ns#"
     xmlns:xml="http://www.w3.org/XML/1998/namespace"
     xmlns:xsd="http://www.w3.org/2001/XMLSchema#"
     xmlns:prov="http://www.w3.org/ns/prov#"
     xmlns:rdfs="http://www.w3.org/2000/01/rdf-schema#"
     xmlns:vann="http://purl.org/vocab/vann/"
     xmlns:terms="http://purl.org/dc/terms/">
    <owl:Ontology rdf:about="https://www.w3id.org/iSeeOnto/BehaviourTreeExecution">
        <owl:imports rdf:resource="http://www.w3.org/ns/prov-o-20130430"/>
        <owl:imports rdf:resource="https://www.w3id.org/iSeeOnto/BehaviourTree"/>
    </owl:Ontology>
    


    <!-- 
    ///////////////////////////////////////////////////////////////////////////////////////
    //
    // Object Properties
    //
    ///////////////////////////////////////////////////////////////////////////////////////
     -->

    


    <!-- https://www.w3id.org/iSeeOnto/BehaviourTreeExecution#enacted -->

    <owl:ObjectProperty rdf:about="https://www.w3id.org/iSeeOnto/BehaviourTreeExecution#enacted">
        <rdfs:subPropertyOf rdf:resource="http://www.w3.org/ns/prov#used"/>
        <rdfs:domain rdf:resource="https://www.w3id.org/iSeeOnto/BehaviourTreeExecution#NodeExecution"/>
        <rdfs:range rdf:resource="https://www.w3id.org/iSeeOnto/BehaviourTree#Node"/>
        <rdfs:comment xml:lang="en">
			This property captures the relationship between a Node (from a Tree in the BehaviourTree ontology) and the NodeExecution prov:Activity that is enacting / executing that Node (viewed as a step in the plan).
		</rdfs:comment>
        <rdfs:label xml:lang="en">enacted</rdfs:label>
    </owl:ObjectProperty>
    


    <!-- https://www.w3id.org/iSeeOnto/BehaviourTreeExecution#outcome -->

    <owl:ObjectProperty rdf:about="https://www.w3id.org/iSeeOnto/BehaviourTreeExecution#outcome">
        <rdfs:subPropertyOf rdf:resource="http://www.w3.org/ns/prov#generated"/>
        <owl:inverseOf rdf:resource="https://www.w3id.org/iSeeOnto/BehaviourTreeExecution#wasOutcomeOf"/>
        <rdfs:domain rdf:resource="https://www.w3id.org/iSeeOnto/BehaviourTreeExecution#NodeExecution"/>
        <rdfs:range rdf:resource="https://www.w3id.org/iSeeOnto/BehaviourTreeExecution#NodeExecutionSuccessIndicator"/>
        <rdfs:comment xml:lang="en">
        This property links a NodeExecution activity to a NodeExecutionSuccessIndicator entity, indicating the outcome of the execution of the Behaviour Tree node.
    </rdfs:comment>
        <rdfs:label xml:lang="en">outcome</rdfs:label>
    </owl:ObjectProperty>
    


    <!-- https://www.w3id.org/iSeeOnto/BehaviourTreeExecution#wasOutcomeOf -->

    <owl:ObjectProperty rdf:about="https://www.w3id.org/iSeeOnto/BehaviourTreeExecution#wasOutcomeOf">
        <rdfs:subPropertyOf rdf:resource="http://www.w3.org/ns/prov#wasGeneratedBy"/>
        <rdfs:domain rdf:resource="https://www.w3id.org/iSeeOnto/BehaviourTreeExecution#NodeExecutionSuccessIndicator"/>
        <rdfs:range rdf:resource="https://www.w3id.org/iSeeOnto/BehaviourTreeExecution#NodeExecution"/>
        <rdfs:comment xml:lang="en">
        This property links a NodeExecutionSuccessIndicator entity to a NodeExecution activity, indicating that the entity is the outcome of the execution of the Behaviour Tree node.
    </rdfs:comment>
        <rdfs:label xml:lang="en">was Outcome Of</rdfs:label>
    </owl:ObjectProperty>
    


    <!-- 
    ///////////////////////////////////////////////////////////////////////////////////////
    //
    // Classes
    //
    ///////////////////////////////////////////////////////////////////////////////////////
     -->

    


    <!-- https://www.w3id.org/iSeeOnto/BehaviourTree#Node -->

    <rdf:Description rdf:about="https://www.w3id.org/iSeeOnto/BehaviourTree#Node">
        <rdfs:subClassOf rdf:resource="http://www.w3.org/ns/prov#Entity"/>
    </rdf:Description>
    


    <!-- https://www.w3id.org/iSeeOnto/BehaviourTree#Tree -->

    <rdf:Description rdf:about="https://www.w3id.org/iSeeOnto/BehaviourTree#Tree">
        <rdfs:subClassOf rdf:resource="http://www.w3.org/ns/prov#Plan"/>
    </rdf:Description>
    


    <!-- https://www.w3id.org/iSeeOnto/BehaviourTreeExecution#NodeExecution -->

    <owl:Class rdf:about="https://www.w3id.org/iSeeOnto/BehaviourTreeExecution#NodeExecution">
        <rdfs:subClassOf rdf:resource="http://www.w3.org/ns/prov#Activity"/>
        <rdfs:subClassOf>
            <owl:Restriction>
                <owl:onProperty rdf:resource="https://www.w3id.org/iSeeOnto/BehaviourTreeExecution#outcome"/>
                <owl:qualifiedCardinality rdf:datatype="http://www.w3.org/2001/XMLSchema#nonNegativeInteger">1</owl:qualifiedCardinality>
                <owl:onClass rdf:resource="https://www.w3id.org/iSeeOnto/BehaviourTreeExecution#NodeExecutionSuccessIndicator"/>
            </owl:Restriction>
        </rdfs:subClassOf>
        <rdfs:comment xml:lang="en">
        An activity that enacts or executes a Behaviour Tree Node over a period of time. The result of executing a Behaviour Tree Node must reference exactly one NodeExecutionSuccessIndicator, which is a prov:Entity that indicates whether the execution was successful or not using the outcome relationship.
    </rdfs:comment>
        <rdfs:label xml:lang="en">Node Execution</rdfs:label>
    </owl:Class>
    


    <!-- https://www.w3id.org/iSeeOnto/BehaviourTreeExecution#NodeExecutionOutput -->

    <owl:Class rdf:about="https://www.w3id.org/iSeeOnto/BehaviourTreeExecution#NodeExecutionOutput">
        <rdfs:subClassOf rdf:resource="http://www.w3.org/ns/prov#Entity"/>
        <rdfs:subClassOf>
            <owl:Restriction>
                <owl:onProperty rdf:resource="https://www.w3id.org/iSeeOnto/BehaviourTree#properties"/>
                <owl:maxQualifiedCardinality rdf:datatype="http://www.w3.org/2001/XMLSchema#nonNegativeInteger">1</owl:maxQualifiedCardinality>
                <owl:onClass rdf:resource="https://www.w3id.org/iSeeOnto/BehaviourTree#Dictionary"/>
            </owl:Restriction>
        </rdfs:subClassOf>
    </owl:Class>
    


    <!-- https://www.w3id.org/iSeeOnto/BehaviourTreeExecution#NodeExecutionSuccessIndicator -->

    <owl:Class rdf:about="https://www.w3id.org/iSeeOnto/BehaviourTreeExecution#NodeExecutionSuccessIndicator">
        <rdfs:subClassOf rdf:resource="http://www.w3.org/ns/prov#Entity"/>
        <rdfs:subClassOf>
            <owl:Restriction>
                <owl:onProperty rdf:resource="http://www.w3.org/ns/prov#value"/>
                <owl:maxQualifiedCardinality rdf:datatype="http://www.w3.org/2001/XMLSchema#nonNegativeInteger">1</owl:maxQualifiedCardinality>
                <owl:onDataRange rdf:resource="http://www.w3.org/2001/XMLSchema#boolean"/>
            </owl:Restriction>
        </rdfs:subClassOf>
    </owl:Class>
</rdf:RDF>



<!-- Generated by the OWL API (version 4.5.9.2019-02-01T07:24:44Z) https://github.com/owlcs/owlapi -->

