@prefix : <http://www.w3id.org/iSeeOnto/workflow#> .
@prefix owl: <http://www.w3.org/2002/07/owl#> .
@prefix rdf: <http://www.w3.org/1999/02/22-rdf-syntax-ns#> .
@prefix xml: <http://www.w3.org/XML/1998/namespace> .
@prefix xsd: <http://www.w3.org/2001/XMLSchema#> .
@prefix rdfs: <http://www.w3.org/2000/01/rdf-schema#> .
@base <http://www.w3id.org/iSeeOnto/workflow> .

<http://www.w3id.org/iSeeOnto/workflow> rdf:type owl:Ontology ;
                                         owl:imports <http://www.w3id.org/iSeeOnto/explainer> ,
                                                     <https://purl.org/heals/eo/1.0.0> ;
                                         <http://purl.org/dc/terms/contributor> "Anjana Wijekoon" ,
                                                                                "Chamath Palihawadana" ,
                                                                                "David Corsar" ,
                                                                                "Ikechukwu Nkisi-Orji" ,
                                                                                "Juan A. Recio-Garcia" ,
                                                                                "Marta Caro Martínez" ;
                                         <http://purl.org/dc/terms/description> """The Workflow Ontology is an ontology provides a high-level description of how an Explainer can be integrated with an eo:AI Method, to generate an ex:Explanation provided to, and evaluated by a eo:User. The representation itself is influenced those of Recio-García (2007) and Garijo (2012) to provide the starting point, which will be extended with more specific types of Tasks (e.g., choice, repeat-while, repeat-until) and parameters (e.g., for describing the passing of parameters for web service calls or programming language - Java, Python, Javascript, etc.), method calls and parameter exchange as required by the use cases.
		
		This representation is influenced by those described by: Recio-García, J., Díaz-Agudo, B., and González-Calero, P. (2009). Semantic templates for case-based reasoning systems. The Knowledge Engineering Review, 24(3), 245-264. doi:10.1017/S0269888909990051; and Garijo D, Gil Y. Augmenting PROV with Plans in P-PLAN: Scientific Processes as Linked Data. Linked Science 2012 - Tackling Big Data workshop ISWC 2012.
		
		This ontology was created as part of the iSee project (https://isee4xai.com) which received funding from EPSRC under the grant number EP/V061755/1. iSee is part of the CHIST-ERA pathfinder programme for European coordinated research on future and emerging information and communication technologies.
		""" ;
                                         <http://purl.org/dc/terms/title> "The Workflow Ontology" ;
                                         <http://purl.org/vocab/vann/preferredNamespacePrefix> "wf" ;
                                         <http://purl.org/vocab/vann/preferredNamespaceUri> "https://www.w3id.org/iSeeOnto/workflow" .

#################################################################
#    Object Properties
#################################################################

###  http://www.w3id.org/iSeeOnto/workflow#composedOf
:composedOf rdf:type owl:ObjectProperty ;
            rdfs:comment "Link between a CompositeTask and the ControlConstruct it is decomposed to." ;
            rdfs:label "composed of"@en .


###  http://www.w3id.org/iSeeOnto/workflow#hasOutput
:hasOutput rdf:type owl:ObjectProperty ;
           rdfs:comment "Link between a Task and a variable generated as output of the Task." ;
           rdfs:label "has output"@en .


###  http://www.w3id.org/iSeeOnto/workflow#isInputTo
:isInputTo rdf:type owl:ObjectProperty ;
           rdfs:comment "Link between a Task and a variable provided as input to the Task." ;
           rdfs:label "is input to"@en .


###  http://www.w3id.org/iSeeOnto/workflow#startTask
:startTask rdf:type owl:ObjectProperty ;
           rdfs:comment "Link between a Workflow and the first task to be performed." ;
           rdfs:label "start task"@en .


#################################################################
#    Classes
#################################################################

###  http://www.w3id.org/iSeeOnto/workflow#CompositeTask
:CompositeTask rdf:type owl:Class ;
               rdfs:subClassOf :Task ,
                               [ rdf:type owl:Restriction ;
                                 owl:onProperty :composedOf ;
                                 owl:someValuesFrom :ControlConstruct
                               ] ;
               rdfs:comment "A Task consisting of a multiple steps. Composite Tasks should be decomposed inot other Tasks through the use of Control Constructs." ;
               rdfs:label "Composite Task"@en .


###  http://www.w3id.org/iSeeOnto/workflow#ControlConstruct
:ControlConstruct rdf:type owl:Class ;
                  rdfs:comment "Defines how multiple tasks should be combined. This is an extension point for the workflow ontology." ;
                  rdfs:label "Control Construct"@en .


###  http://www.w3id.org/iSeeOnto/workflow#IfTheElse
:IfTheElse rdf:type owl:Class ;
           rdfs:subClassOf :ControlConstruct ;
           rdfs:comment "An If-Then-Else control construct to be used to define that a specified Task should be performed if some condition is satified, otherwise another Task should be performed." ;
           rdfs:label "If Then Else"@en .


###  http://www.w3id.org/iSeeOnto/workflow#Sequence
:Sequence rdf:type owl:Class ;
          rdfs:subClassOf :ControlConstruct ;
          rdfs:comment "An Sequence control construct to be used to define a list of Task that should be performed in the specified order." ;
          rdfs:label "Sequence"@en .


###  http://www.w3id.org/iSeeOnto/workflow#SimpleTask
:SimpleTask rdf:type owl:Class ;
            rdfs:subClassOf :Task ;
            rdfs:comment "A Task consisting of a single-step that can be achieved by some method.." ;
            rdfs:label "Simple Task"@en .


###  http://www.w3id.org/iSeeOnto/workflow#Task
:Task rdf:type owl:Class ;
      rdfs:subClassOf [ rdf:type owl:Restriction ;
                        owl:onProperty :hasOutput ;
                        owl:someValuesFrom :Variable
                      ] ;
      rdfs:comment "A Task is a step in a workflow that will be performed to generate an explanation." ;
      rdfs:label "Task"@en .


###  http://www.w3id.org/iSeeOnto/workflow#Variable
:Variable rdf:type owl:Class ;
          rdfs:subClassOf [ rdf:type owl:Restriction ;
                            owl:onProperty :isInputTo ;
                            owl:someValuesFrom :Task
                          ] ;
          rdfs:comment "Variables are used to define parameters that can be passed as input to a Task, or produced as the output of a Task." ;
          rdfs:label "Variable"@en .


###  http://www.w3id.org/iSeeOnto/workflow#Workflow
:Workflow rdf:type owl:Class ;
          rdfs:subClassOf [ rdf:type owl:Restriction ;
                            owl:onProperty :startTask ;
                            owl:someValuesFrom :Task
                          ] ;
          rdfs:comment "A Workflow consists of one or more Tasks to generate an Explanation that will be provided to, and evaluated by, the User. Tasks can be either a SimpleTask representing a single-step that can be achieved by some Method, or a CompositeTask.  " ;
          rdfs:label "Workflow"@en .


###  Generated by the OWL API (version 5.1.14) https://github.com/owlcs/owlapi/
